Proved half of list induction

theories/clang/lib/list.v
@@ -1,32 +1,56 @@
 (* Singly linked list *)
 
 From iris_os.clang Require Import logic tactics notations.
+Require Import lib.gmap_solve.
 
 Section proof.
   Context `{clangG Σ}.
 
   Fixpoint isList (l: val) (xs: list val) (t: type) :=
     match xs with
-      | [] => True%I
+      | [] => (⌜ l = null ⌝)%I
       | x::xs' => (∃ p l',
                      ⌜ l = Vptr p ∧ typeof t x ⌝ ∗
                      p ↦ Vpair x l' @ (Tprod t (Tptr t)) ∗ isList l' xs' t)%I
     end.
 
-  Parameter y t: addr.
+  Parameter y t px: addr.
+  Parameter x: ident.
 
   (* de brujin with autosubst? *)
   Definition tcell (telem: type): type := Tmu 0 (Tprod telem (Tptr (Tvar 0))).
   Definition tlist (telem: type): type := Tptr (tcell telem).
-  
-  Definition rev_list (x: val) (telem: type) : stmts :=
-    y <- null ;;
-    while ( x != null ) {{
-      t <- snd (!x) ;;
-      snd (!x) <- y ;;
-      y <- x ;;
-      x <- t
-    }};;
-    x <- y.
 
+  Definition rev_list (telem: type) : stmts :=
+    y <- null ;;
+    while [ x != null ] ( x != null ) <{
+      t <- snd (!x) ;;
+      snd (!x) <- !y ;;
+      y <- x ;;
+      x <- !t
+    }>;;
+    x <- !y.
+
+  Lemma rev_spec l ety Φ Φret body xs:
+    instantiate_f_body {[ x := (tlist ety, px) ]} (rev_list ety) = Some body →
+    isList l xs ety ∗ y ↦ - ∗ t ↦ - ∗ px ↦ l @ tlist ety ∗
+    (isList l (rev xs) ety -∗ Φ Vvoid)
+    ⊢ WP curs body {{ Φ; Φret }}.
+  Proof.
+    induction xs as [|x xs' IHxs'].
+    - iIntros (?) "(% & Hy & Ht & Hpx & HΦ)".
+      rewrite /instantiate_f_body /resolve_rhs map_to_list_singleton in H0.
+      simpl in H0.
+      destruct (decide (x = x))=>//.
+      destruct px. gmap_solve.
+      iDestruct "Hy" as (??) "Hy".
+      wp_assign. wp_load.
+      wp_op. simpl.
+      iApply wp_while_false.
+      iNext. wp_load. wp_assign.
+      by iApply "HΦ".
+    - 
+    
+    
+  
 End proof.
